feat: Generic traits (#613)
* Add member type checking/inference for generic traits

In the future, traits won't be for just reference types. To try to reduce the number
of dependencies of traits on references, I moved the InheritedMembers, TraitsTyp,
TraitsObj, and the new field ParentFormalTypeParametersToActuals from
ClassDecl into TopLevelDeclWithMembers.

* refactor: Move CheckOverride_* methods from RefinementTransformer into Resolver

* Instantiate formal type parameters of traits with their actual types when compiling

Dafny allows a type parameter of a function/method to shadow a type parameter of the enclosing type. This
does not hold true in all target languages (e.g., C#). The compiler now prepends "_" to the name of any
function/method type parameter, which removes any ambiguities.

The test cases in TraitCompile.dfy now compile correctly for C# and JavaScript.
* Compilation to Java fails, because the tests include a static method that uses a type parameter of the enclosing class. This is not directly supported in Java. The problem is not related to generic traits--it is also a problem in generic classes (that don't extend any trait).
* Compilation to Go fails. This is due to a problem in compiling generic methods.

* fix: bitvector types in traits

Fixes #549

* Add function axioms involving generic traits

* Use class name as value for dtype, not name of non-null type

* chore: Clarify role of `MemberSelectExpression.TypeApplication`

* chore: Rename and explain "nptype" parameter of ResolveMember

* Correct and simplify readsHeap logic

Since `AlwaysUseHeap || f.ReadsHeap ==> readsHeap`, some expressions can be simplified.

The previous expressions `AlwaysUseHeap || f.ReadsHeap || !readsHeap` were incorrect. They should have been

    !(AlwaysUseHeap || f.ReadsHeap || readsHeap)

which, on account of the implication above, is the same as just `!readsHeap`.

* Remove heap argument from function override axiom

Previously, the "pseudo body" of overridden function was consulted to see if the heap was used.

* Improve trigger of function override axiom

* Fix up parameters to functions in override axiom

* Fix problem with only-provided imports of generic traits

* refactor: Break off FunctionOverrideAxiom from FunctionAxiom

* Fix type parameters in function/method override checks

* Translate const fields with appropriate type parameters

* Fix `MemberSelectExpr.TypeApplication` initialization in constructor from `Field`

* Rename `DerivesFrom` to `HeadDerivesFrom`

* refactor: Rename `TopLevelDeclWithMembers.TraitObj` to `TraitParentHeads`

* Check for duplicate parent traits with different type arguments

* refactor: Rename `TraitsTyp` to `ParentTypes`

* refactor: Rename `TraitParentHeads` to `ParentTraitHeads`

* fix: Don't allow overrides of static members

* fix: Check agreement on ghost etc. of overridden members

* Improve wording of error messages

* fix: Axiomatize "extends" relation on classes and traits

* Replace `MemberSelectExpr.TypeApplication` and `FunctionCallExpr.TypeArgumentSubstitutions` with `TypeApplication_*` fields and clarify the meaning

* fix: Substitution into `StaticReceiverExpr` to do type substitution.

* fix: Make sure `ArrowType.ResolvedClass` is filled in

* Reword error messages about not being able to determine types and about type-parameter characteristics

* chore: Remove unused parameters of `Translator.RecursiveCallParameters`

* Replace some uses of `TypeArgumentSubstitutionsWithParents()` with `TypeApplication_JustMember`

Co-authored-by: Robin Salkeld <salkeldr@amazon.com>

Source/Dafny/Cloner.cs
@@ -107,7 +107,7 @@ namespace Microsoft.Dafny
         if (d is DefaultClassDecl) {
           return new DefaultClassDecl(m, mm);
         } else {
-          return new ClassDecl(Tok(dd.tok), dd.Name, m, tps, mm, CloneAttributes(dd.Attributes), dd.TraitsTyp.ConvertAll(CloneType));
+          return new ClassDecl(Tok(dd.tok), dd.Name, m, tps, mm, CloneAttributes(dd.Attributes), dd.ParentTraits.ConvertAll(CloneType));
         }
       } else if (d is ModuleDecl) {
         if (d is LiteralModuleDecl) {
