Test/hofs/Naked.dfy
@@ -19,11 +19,11 @@ module Functions {
 
 module Requires {
   function t(x: nat): nat
-  requires !t.requires(x);  // error: use of naked function in its own SCC
+    requires !t.requires(x);  // error: use of naked function in its own SCC
   { x }
 
   function g(x: nat): nat
-  requires !(g).requires(x);  // error: use of naked function in its own SCC
+    requires !(g).requires(x);  // error: use of naked function in its own SCC
   { x }
 
   function D(x: int): int  // used so termination errors don't mask other errors
@@ -35,17 +35,36 @@ module Requires {
 
 module Reads {
   function t(x: nat): nat
-  reads t.reads(x);
+    reads t.reads(x);
   { x }
 
   function g(x: nat): nat
-  reads (g).reads(x);
+    reads (g).reads(x);
   { x }
 
-  function g2(x: int): int { h(x) }
+  function g2(x: int): int
+  { h(x) }
 
   function h(x: int): int
     reads g2.reads(x);
   { x }
 }
 
+module ReadsGenerics {
+  class Cl<A> {
+    function t<B>(a: A, b: B): (A, B)
+      reads t.reads(a, b);
+    { (a, b) }
+
+    function g<B>(a: A, b: B): (A, B)
+      reads (g).reads(a, b);
+    { (a, b) }
+
+    function g2<B>(a: A, b: B): (A, B)
+    { h(a, b) }
+
+    function h<B>(a: A, b: B): (A, B)
+      reads g2.reads(a, b);
+    { (a, b) }
+  }
+}
