Test/git-issues/git-issue-549.dfy
@@ -1,0 +1,20 @@
+// RUN: %dafny /compile:3 "%s" > "%t"
+// RUN: %diff "%s.expect" "%t"
+
+trait T {
+  function method bar(): bv8
+}
+
+class F extends T {
+  // once upon a time, the following used to crash Dafny
+  function method bar(): bv8 {
+    1
+  }
+}
+
+method Main() {
+  var f: F := new F;
+  print "bar() = ", f.bar(), "\n";
+  var t: T := new F;
+  print "bar() = ", t.bar(), "\n";
+}
